restructure

code/theories/Reduction.v
@@ -1,81 +1,186 @@
-From Interpolation Require Import Utils Syntax.
-From Stdlib Require Import Relations Arith Lia Bool List RelationClasses.
+From Interpolation Require Import Utils Syntax Notations.
+From Stdlib Require Import Setoid Morphisms Relation_Definitions RelationClasses.
+From Stdlib Require Import Relations Arith Lia Bool List.
 
 Import ListNotations.
 
 (** ** Reduction *)
 
-Reserved Notation "t '-->' t'" (at level 40).
+Section Reduction.
+  Close Scope typing_scope.
 
-Inductive step : term -> term -> Prop :=
-  | ST_Beta t1 v2 :
-        tApp (tLam t1) v2 --> t1[v2..]
-  | ST_App_l t1 t1' t2 :
-         t1 --> t1' ->
-         tApp t1 t2 --> tApp t1' t2
-  | ST_App_r t1 t2 t2' :
-         t2 --> t2' ->
-         tApp t1 t2 --> tApp t1 t2'
-  | ST_Lam t t' :
-    t --> t' ->
-    tLam t --> tLam t'
-  | ST_Fst t t' : tFst (tPair t t') --> t
-  | ST_Snd t t' : tSnd (tPair t t') --> t'
-  | ST_Proj b t t' :
-         t --> t' ->
-         tProj b t --> tProj b t'
-  | ST_Pair_l t1 t1' t2 :
-         t1 --> t1' ->
-         tPair t1 t2 --> tPair t1' t2
-  | ST_Par_r t1 t2 t2' :
-         t2 --> t2' ->
-         tPair t1 t2 --> tPair t1 t2'
+  Inductive term_ored : relation term :=
+    | ST_Beta t1 v2 :
+          tApp (tLam t1) v2 ⤳ t1[v2..]
+    | ST_App_l t1 t1' t2 :
+          t1 ⤳ t1' ->
+          tApp t1 t2 ⤳ tApp t1' t2
+    | ST_App_r t1 t2 t2' :
+          t2 ⤳ t2' ->
+          tApp t1 t2 ⤳ tApp t1 t2'
+    | ST_Lam t t' :
+      t ⤳ t' ->
+      tLam t ⤳ tLam t'
+    | ST_Fst t t' : tFst (tPair t t') ⤳ t
+    | ST_Snd t t' : tSnd (tPair t t') ⤳ t'
+    | ST_Proj b t t' :
+          t ⤳ t' ->
+          tProj b t ⤳ tProj b t'
+    | ST_Pair_l t1 t1' t2 :
+          t1 ⤳ t1' ->
+          tPair t1 t2 ⤳ tPair t1' t2
+    | ST_Par_r t1 t2 t2' :
+          t2 ⤳ t2' ->
+          tPair t1 t2 ⤳ tPair t1 t2'
 
-where "t '-->' t'" := (step t t').
+  where "t '⤳' t'" := (term_ored t t').
 
-Hint Constructors step : core.
+End Reduction.
 
-Notation multistep := (clos_refl_trans term step).
-Notation "t1 '-->*' t2" := (multistep t1 t2) (at level 40).
+Hint Constructors term_ored : core.
 
-Instance red_po : PreOrder multistep.
-Proof.
-  constructor.
-  all: now econstructor.
-Qed.
+Notation term_red := (clos_refl_trans term term_ored).
 
-Lemma R_App_cong f f' u u':
-  f -->* f' ->
-  u -->* u' ->
-  tApp f u -->* tApp f' u'.
-Proof.
-  intros Hf Hu.
-  induction Hf using clos_refl_trans_ind_left ; eauto using rt_refl, rt_step, rt_trans.
-  induction Hu using clos_refl_trans_ind_left ; eauto using rt_refl, rt_step, rt_trans.
-Qed.
+#[export] Instance HasORedTm : HasORed term := term_ored.
+#[export] Instance HasRedTm : HasRed term := term_red.
 
-Lemma R_Lam_cong t t':
-  t -->* t' ->
-  tLam t -->* tLam t'.
-Proof.
-  intros Ht.
-  induction Ht using clos_refl_trans_ind_left ; eauto using rt_refl, rt_step, rt_trans.
-Qed.
 
-Lemma R_Proj_cong b t t' :
-  t -->* t' ->
-  tProj b t -->* tProj b t'.
-Proof.
-  intros Hred.
-  induction Hred using clos_refl_trans_ind_left ; eauto using rt_refl, rt_step, rt_trans.
-Qed.
+Definition subst_red : relation subst :=
+  fun σ τ => forall i, σ i ⤳* τ i.
 
-Lemma R_Pair_cong p p' q q':
-  p -->* p' ->
-  q -->* q' ->
-  tPair p q -->* tPair p' q'.
-Proof.
-  intros Hp Hq.
-  induction Hp using clos_refl_trans_ind_left ; eauto using rt_refl, rt_step, rt_trans.
-  induction Hq using clos_refl_trans_ind_left ; eauto using rt_refl, rt_step, rt_trans.
-Qed.
+#[export] Instance HasRedSubst : HasRed subst := subst_red.
+
+  Ltac fold_red :=
+    change term_ored with ored in * ;
+    change term_red with red in * ;
+    change subst_red with red in *.
+
+  Smpl Add fold_red : refold.
+
+Section Properties.
+  #[local] Notation red := (Notations.red (Obj := term)) (only parsing).
+  #[local] Notation sred := (Notations.red (Obj := subst)) (only parsing).
+
+  Instance red_po : PreOrder red.
+  Proof.
+    constructor.
+    all: now econstructor.
+  Qed.
+
+  Instance R_App_cong :
+    Proper (red ==> red ==> red) tApp.
+  Proof.
+    intros ?? Hf ?? Hu ; unfold Notations.red, HasRedTm in *.
+    induction Hf using clos_refl_trans_ind_left ; eauto using rt_refl, rt_step, rt_trans.
+    induction Hu using clos_refl_trans_ind_left ; eauto using rt_refl, rt_step, rt_trans.
+  Qed.
+
+  Instance R_Lam_cong : Proper (red ==> red) tLam.
+  Proof.
+    intros ?? Ht ; unfold Notations.red, HasRedTm in *.
+    induction Ht using clos_refl_trans_ind_left ; eauto using rt_refl, rt_step, rt_trans.
+  Qed.
+
+  Instance R_Proj_cong : Proper (eq ==> red ==> red) tProj.
+  Proof.
+    intros ?? -> ?? Hred ; unfold Notations.red, HasRedTm in *.
+    induction Hred using clos_refl_trans_ind_left ; eauto using rt_refl, rt_step, rt_trans.
+  Qed.
+
+  Instance R_Pair_cong : Proper (red ==> red ==> red) tPair.
+  Proof.
+    intros ?? Hp ?? Hq ; unfold Notations.red, HasRedTm in *.
+    induction Hp using clos_refl_trans_ind_left ; eauto using rt_refl, rt_step, rt_trans.
+    induction Hq using clos_refl_trans_ind_left ; eauto using rt_refl, rt_step, rt_trans.
+  Qed.
+
+  Instance ST_ren : Proper ((pointwise_relation _ eq) ==> ored ==> ored) ren1.
+  Proof.
+    intros ρ ρ' Hren t t' Ht.
+    rewrite <- Hren ; clear ρ' Hren.
+    induction Ht in ρ |- * ; cbn ; try solve [now constructor].
+    replace (_[_]⟨_⟩) with ((t1⟨upRen_term_term ρ⟩[v2⟨ρ⟩..])).
+    1: constructor.
+    now substify ; asimpl.
+  Qed.
+
+  Instance R_ren : Proper ((pointwise_relation _ eq) ==> red ==> red) ren1.
+  Proof.
+    intros ρ ρ' Hren t t' Ht.
+    rewrite <- Hren ; clear ρ' Hren.
+    induction Ht.
+    all: try solve [now econstructor].
+    econstructor.
+    now apply ST_ren.
+  Qed.
+
+  Lemma R_lift : Proper (sred ==> sred) up_term_term.
+  Proof.
+    intros ?? ? [|] ; cbn.
+    - reflexivity.
+    - rewrite R_ren ; try reflexivity.
+      auto.
+  Qed.
+
+  Instance R_subst_same : Proper (sred ==> @eq term ==> red) subst1.
+  Proof.
+    intros σ τ Hsubst ? t ->.
+    induction t in σ, τ, Hsubst |- * ; cbn.
+    - apply Hsubst.
+    - reflexivity.
+    - erewrite IHt1, IHt2 ; tea ; reflexivity.
+    - rewrite IHt ; tea ; reflexivity.
+    - rewrite IHt.
+      1: reflexivity.
+      now apply R_lift.
+    - erewrite IHt1, IHt2 ; tea ; reflexivity.
+  Qed.
+
+  Instance R_cons : Proper (red ==> sred ==> sred) scons.
+  Proof.
+    intros ?? Ht ?? Hσ [|] ; now cbn.
+  Qed.
+
+  Instance R_subst : Proper (sred ==> ored (Obj := term) ==> red) subst1.
+  Proof.
+    intros σ σ' Hsubst t t' Ht.
+    induction Ht in σ, σ', Hsubst |- * ; cbn.
+    - etransitivity.
+      1: do 2 constructor.
+      asimpl ; refold.
+      apply R_subst_same ; eauto.
+      apply R_cons ; eauto.
+      rewrite R_subst_same ; eauto ; reflexivity.
+    - erewrite IHHt ; tea.
+      apply R_App_cong ; try easy.
+      rewrite R_subst_same ; try easy.
+      easy.
+    - erewrite IHHt ; tea.
+      apply R_App_cong ; try easy.
+      rewrite R_subst_same ; try easy.
+      easy.
+    - erewrite IHHt.
+      2:{ now apply R_lift. }
+      now apply R_Lam_cong.
+    - etransitivity.
+      1: do 2 constructor.
+      now apply R_subst_same.
+    - etransitivity.
+      1: do 2 constructor.
+      now apply R_subst_same.
+    - erewrite IHHt ; tea.
+      now apply R_Proj_cong.
+    - erewrite IHHt ; tea.
+      apply R_Pair_cong ; try easy.
+      rewrite R_subst_same ; try easy.
+      easy.
+     - erewrite IHHt ; tea.
+      apply R_Pair_cong ; try easy.
+      rewrite R_subst_same ; try easy.
+      easy.
+  Qed.
+
+End Properties.
+
+Existing Instances red_po R_App_cong R_Lam_cong R_Proj_cong R_Pair_cong R_ren
+  R_lift R_cons R_subst.
