code/theories/Context.v
@@ -1,0 +1,29 @@
+From Stdlib Require Import List.
+From Interpolation Require Import Ast.
+
+Import ListNotations.
+
+Fixpoint nth_error {A} (l : list A) (n : nat) : option A :=
+  match l, n with
+  | nil, _ => None
+  | a :: _, 0 => Some a
+  | _ :: l', S n' => nth_error l' n'
+  end.
+
+(** ** Typing *)
+
+Definition context := list type.
+
+Notation "'ε'" := (@nil type).
+Notation "Γ ,,, T" := (@cons type T Γ) (at level 50).
+(* 
+Notation "'ε'" := (nil :> context) (only parsing).
+Notation "Γ ,,, T" := (cons T Γ :> context) (at level 50, only parsing). *)
+
+Definition in_context (n : nat) (Γ : context) (T : type) : Prop :=
+  nth_error Γ n = Some T.
+
+Lemma in_zero Γ T : in_context 0 (Γ,,,T) T.
+Proof. reflexivity. Qed.
+
+Hint Resolve in_zero : core.
