code/theories/Notations.v
@@ -1,0 +1,20 @@
+From Interpolation Require Import Utils Syntax Context.
+From Stdlib Require Import Relation_Definitions.
+
+Declare Scope typing_scope.
+Delimit Scope typing_scope with ty.
+
+Open Scope typing_scope.
+
+Class HasTyping (Ctx Ty Obj : Type) := typing : Ctx -> Ty -> Obj -> Prop.
+Class HasRed (Obj : Type) := red : relation Obj.
+Class HasORed (Obj : Type) := ored : relation Obj.
+
+(** The object t has type A in Γ *)
+Notation "Γ '|-' t '::' T" := (typing Γ T t)
+  (at level 101, t at level 59) : typing_scope.
+
+(** Term t one-step reduces to term t' *)
+Notation "t '⤳' t'" := (ored t t') (at level 40) : typing_scope.
+(** Term t multi-step reduces to term t' *)
+Notation "t '⤳*' t'" := (red t t') (at level 40) : typing_scope.
